# Euler's identity

$$
e^{i\pi}+1=0
$$

$$
e^{i\pi}+1-1=0-1,\:Thus\:e^{i\pi}=-1
$$

The beauty of this formula is the what it actually does. It connects e; the base of the natural log, i; the imaginary 1D basis vector unit, 1; the multiplicative constant, and 0; the the addictive constant. Euler's identity can be expanded to the following:



$$
\left(1+\frac{1}{n}\right)^{\left(n\cdot\sqrt{-1}\cdot\sum_{k=0}^{\infty}\frac{\left(-1\right)^{k}}{2k+1}\right)}
$$

$$
e^{i\pi}+1=0
$$

$$
e^i
$$

$$
f(x) = x * e^{2 pi i \xi x}
$$

